feat(TM): sketch simple Write TM, show properties

Primitive_TMs.thy
@@ -40,7 +40,8 @@ locale read_TM = TM "Abs_TM (read_TM_rec k \<Sigma>)"
     and nonempty_symbols: "\<Sigma> \<noteq> {}"
 begin
 
-lemma M_rec: "M_rec = read_TM_rec k \<Sigma>" using read_TM_rec_valid[OF at_least_one_tape finite_symbols nonempty_symbols]
+lemma M_rec: "M_rec = read_TM_rec k \<Sigma>"
+  using read_TM_rec_valid[OF at_least_one_tape finite_symbols nonempty_symbols]
   by (intro Abs_TM_inverse CollectI)
 
 lemma M_fields:
@@ -61,17 +62,14 @@ declare M_fields(1-6)[simp]
 lemma step:
   assumes "state c = q\<^sub>0"
     and "wf_config c"
-  shows "step c = TM_config (Some (head (hd (tapes c)))) (tapes c)"
-  using assms
+  shows "step c = TM_config (Some (head (hd (tapes c)))) (tapes c)" using assms
 proof (induction c)
   case (TM_config q tps)
   let ?c = "TM_config q tps"
   let ?h = "head (hd tps)"
 
-  assume "state ?c = q\<^sub>0"
-  then have [simp]: "q = q\<^sub>0" by simp
-  assume "wf_config ?c"
-  from wf_configD(2)[OF this] have [simp]: "length tps = tape_count" by simp
+  from \<open>state ?c = q\<^sub>0\<close> have [simp]: "q = q\<^sub>0" by simp
+  from wf_configD(2)[OF \<open>wf_config ?c\<close>] have [simp]: "length tps = tape_count" by simp
   from \<open>wf_config ?c\<close> have "tps \<noteq> []" by force
 
   have "step ?c = step_not_final ?c" by force
@@ -110,5 +108,120 @@ proof -
 qed
 
 end \<comment> \<open>\<^locale>\<open>read_TM\<close>\<close>
+
+
+definition write_TM_rec :: "'s option \<Rightarrow> nat \<Rightarrow> 's set \<Rightarrow> (bool, 's, unit) TM_record"
+  where "write_TM_rec \<sigma> k \<Sigma> \<equiv> \<lparr>
+    TM_record.tape_count = k,
+    symbols = \<Sigma>,
+    states = UNIV,
+    initial_state = False,
+    final_states = {True},
+    label = \<lambda>q. (),
+    next_state = \<lambda>q hds. True,
+    next_write = \<lambda>q hds i. if i = 0 then \<sigma> else hds ! i,
+    next_move  = \<lambda>q hds i. No_Shift
+  \<rparr>"
+
+lemma write_TM_rec_valid:
+  assumes "k > 0"
+    and "finite \<Sigma>"
+    and "\<Sigma> \<noteq> {}"
+    and "\<sigma> \<in> options \<Sigma>"
+  shows "valid_TM (write_TM_rec \<sigma> k \<Sigma>)" unfolding write_TM_rec_def
+proof (intro valid_TM_I)
+  show "finite (UNIV :: bool set)" by simp
+
+  fix q hds i
+  assume "hds ! i \<in> options \<Sigma>"
+  with \<open>\<sigma> \<in> options \<Sigma>\<close> show "(if i = 0 then \<sigma> else hds ! i) \<in> options \<Sigma>" by (cases rule: ifI) blast
+qed (use assms in blast)+
+
+
+
+definition "write_TM_M \<sigma> k \<Sigma> \<equiv> Abs_TM (write_TM_rec \<sigma> k \<Sigma>)"
+
+locale write_TM = TM "Abs_TM (write_TM_rec \<sigma> k \<Sigma>)"
+  for \<sigma> :: "'s option" and k :: nat and \<Sigma> :: "'s set" +
+  assumes at_least_one_tape: "k > 0"
+    and finite_symbols: "finite \<Sigma>"
+    and nonempty_symbols: "\<Sigma> \<noteq> {}"
+    and write_valid: "\<sigma> \<in> options \<Sigma>"
+begin
+
+lemma M_rec: "M_rec = write_TM_rec \<sigma> k \<Sigma>"
+  using write_TM_rec_valid[OF at_least_one_tape finite_symbols nonempty_symbols write_valid]
+  by (intro Abs_TM_inverse CollectI)
+
+lemma M_fields:
+  shows "tape_count \<equiv> k"
+    and "symbols \<equiv> \<Sigma>"
+    and "Q \<equiv> UNIV"
+    and "q\<^sub>0 \<equiv> False"
+    and "F \<equiv> {True}"
+    and "label \<equiv> \<lambda>q. ()"
+    and "\<delta>\<^sub>q \<equiv> \<lambda>q hds. True"
+    and "\<delta>\<^sub>w \<equiv> \<lambda>q hds i. (if i = 0 then \<sigma> else hds ! i)"
+    and "\<delta>\<^sub>m \<equiv> \<lambda>q hds i. No_Shift"
+  unfolding TM_fields_defs M_rec unfolding write_TM_rec_def TM_record.simps .
+
+declare M_fields(2-6)[simp]
+
+
+lemma step:
+  assumes "state c = q\<^sub>0"
+    and "wf_config c"
+  shows "step c = TM_config True (tape_write \<sigma> (hd (tapes c)) # tl (tapes c))" using assms
+proof (induction c)
+  case (TM_config q tps)
+  let ?c = "TM_config q tps"
+    and ?h = "head (hd tps)"
+    and ?tps' = "tape_write \<sigma> (hd tps) # tl tps"
+
+  from \<open>state ?c = q\<^sub>0\<close> have [simp]: "q = q\<^sub>0" by simp
+  from wf_configD(2)[OF \<open>wf_config ?c\<close>] have [simp]: "length tps = tape_count" by simp
+  from \<open>wf_config ?c\<close> have "tps \<noteq> []" by force
+
+  have "step ?c = step_not_final ?c" by force
+  also have "... = TM_config True ?tps'"
+  proof (rule TM_config_eq, unfold step_not_final_simps TM_config.sel)
+    let ?hds = "map head tps"
+    show "\<delta>\<^sub>q q ?hds = True" unfolding M_fields ..
+
+    from \<open>tps \<noteq> []\<close> show "map2 tape_action (\<delta>\<^sub>a q ?hds) tps = ?tps'"
+    proof (intro step_not_final_eqI, unfold length_Cons)
+      from \<open>length tps = tape_count\<close> show "Suc (length (tl tps)) = tape_count" by simp
+
+      fix i
+      assume "i < tape_count"
+      then show "tape_action (\<delta>\<^sub>w q ?hds i, \<delta>\<^sub>m q ?hds i) (tps ! i) = ?tps' ! i"
+      proof (induction i)
+        case 0
+        with \<open>tps \<noteq> []\<close> show ?case unfolding M_fields by (simp add: if_P hd_conv_nth)
+      next
+        case (Suc i)
+        from \<open>Suc i < tape_count\<close> have "Suc i < length tps" by simp
+        then have "i < length (tl tps)" unfolding length_tl less_diff_conv by simp
+        from nth_tl[OF this] and \<open>Suc i < length tps\<close> show ?case unfolding M_fields by simp
+      qed
+    qed auto
+  qed
+  finally show ?case unfolding TM_config.sel .
+qed
+
+
+lemma
+  assumes "state c = q\<^sub>0"
+    and "wf_config c"
+  shows "is_final (step c)"
+    and "head (hd (tapes (step c))) = \<sigma>"
+proof -
+  have [simp]: "tapes (step c) = tape_write \<sigma> (hd (tapes c)) # tl (tapes c)" unfolding step[OF assms] by simp
+  have [simp]: "state (step c) = True" unfolding step[OF assms] by simp
+  show "is_final (step c)" unfolding is_final_def by simp
+
+  show "head (hd (tapes (step c))) = \<sigma>" by simp
+qed
+
 
 end
